FOL/NV/Prop.lean
@@ -7,7 +7,7 @@ set_option autoImplicit false
 
 namespace FOL.NV
 
-open Formula
+open Formula_
 
 open Margaris
 
@@ -17,31 +17,31 @@ axiom def_false_ : false_ = not_ true_
 /--
   phi ∨ psi := ¬ phi → psi
 -/
-axiom def_or_ (phi psi : Formula) : or_ phi psi = (not_ phi).imp_ psi
+axiom def_or_ (phi psi : Formula_) : or_ phi psi = (not_ phi).imp_ psi
 
 /--
 phi ∧ psi := ¬ ( phi → ¬ psi )
 -/
-axiom def_and_ (phi psi : Formula) : and_ phi psi = not_ (phi.imp_ (not_ psi))
+axiom def_and_ (phi psi : Formula_) : and_ phi psi = not_ (phi.imp_ (not_ psi))
 
 /--
   phi ↔ psi := ( phi → psi ) ∧ ( psi → phi )
 -/
-axiom def_iff_ (phi psi : Formula) : iff_ phi psi = (phi.imp_ psi).and_ (psi.imp_ phi)
+axiom def_iff_ (phi psi : Formula_) : iff_ phi psi = (phi.imp_ psi).and_ (psi.imp_ phi)
 
 /--
   ∃ x phi := ¬ ∀ x ¬ phi
 -/
-axiom def_exists_ (x : VarName_) (phi : Formula) : exists_ x phi = not_ (forall_ x (not_ phi))
+axiom def_exists_ (x : VarName_) (phi : Formula_) : exists_ x phi = not_ (forall_ x (not_ phi))
 
-def def_eq_ (x y : VarName_) : Formula :=
+def def_eq_ (x y : VarName_) : Formula_ :=
   pred_const_ (PredName_.mk "=") [x, y]
 
 
 /--
   Used for the soundness and completeness proofs of classical propositional logic.
 -/
-def Formula.IsPrime : Formula → Prop
+def Formula_.IsPrime : Formula_ → Prop
   | pred_const_ _ _ => True
   | pred_var_ _ _ => True
   | eq_ _ _ => True
@@ -57,7 +57,7 @@ def Formula.IsPrime : Formula → Prop
   | def_ _ _ => True
 
 
-def Formula.primeSet : Formula → Finset Formula
+def Formula_.primeSet : Formula_ → Finset Formula_
   | pred_const_ X xs => {pred_const_ X xs}
   | pred_var_ X xs => {pred_var_ X xs}
   | eq_ x y => {eq_ x y}
@@ -73,7 +73,7 @@ def Formula.primeSet : Formula → Finset Formula
   | def_ X xs => {def_ X xs}
 
 
-def Formula.substPrime (σ : Formula → Formula) : Formula → Formula
+def Formula_.substPrime (σ : Formula_ → Formula_) : Formula_ → Formula_
   | pred_const_ X xs => σ (pred_const_ X xs)
   | pred_var_ X xs => σ (pred_var_ X xs)
   | eq_ x y => σ (eq_ x y)
@@ -89,21 +89,21 @@ def Formula.substPrime (σ : Formula → Formula) : Formula → Formula
   | def_ X xs => σ (def_ X xs)
 
 
-def VarBoolAssignment := Formula → Bool
+def VarBoolAssignment := Formula_ → Bool
   deriving Inhabited
 
 
-def Formula.evalPrime (V : VarBoolAssignment) : Formula → Prop
+def Formula_.evalPrime (V : VarBoolAssignment) : Formula_ → Prop
   | pred_const_ X xs => V (pred_const_ X xs)
   | pred_var_ X xs => V (pred_var_ X xs)
   | eq_ x y => V (eq_ x y)
   | true_ => True
   | false_ => False
-  | not_ phi => ¬ Formula.evalPrime V phi
-  | imp_ phi psi => Formula.evalPrime V phi → Formula.evalPrime V psi
-  | and_ phi psi => Formula.evalPrime V phi ∧ Formula.evalPrime V psi
-  | or_ phi psi => Formula.evalPrime V phi ∨ Formula.evalPrime V psi
-  | iff_ phi psi => Formula.evalPrime V phi ↔ Formula.evalPrime V psi
+  | not_ phi => ¬ Formula_.evalPrime V phi
+  | imp_ phi psi => Formula_.evalPrime V phi → Formula_.evalPrime V psi
+  | and_ phi psi => Formula_.evalPrime V phi ∧ Formula_.evalPrime V psi
+  | or_ phi psi => Formula_.evalPrime V phi ∨ Formula_.evalPrime V psi
+  | iff_ phi psi => Formula_.evalPrime V phi ↔ Formula_.evalPrime V psi
   | forall_ x phi => V (forall_ x phi)
   | exists_ x phi => V (exists_ x phi)
   | def_ X xs => V (def_ X xs)
@@ -111,61 +111,61 @@ def Formula.evalPrime (V : VarBoolAssignment) : Formula → Prop
 
 instance
   (V : VarBoolAssignment)
-  (F : Formula) :
-  Decidable (Formula.evalPrime V F) :=
+  (F : Formula_) :
+  Decidable (Formula_.evalPrime V F) :=
   by
   induction F generalizing V
   all_goals
-    simp only [Formula.evalPrime]
+    simp only [Formula_.evalPrime]
     infer_instance
 
 
-def Formula.IsTautoPrime (P : Formula) : Prop :=
+def Formula_.IsTautoPrime (P : Formula_) : Prop :=
   ∀ V : VarBoolAssignment, P.evalPrime V
 
 
 def evalPrimeFfToNot
   (V : VarBoolAssignment)
-  (P : Formula) :
-  Formula :=
-  if Formula.evalPrime V P
+  (P : Formula_) :
+  Formula_ :=
+  if Formula_.evalPrime V P
   then P
   else P.not_
 
 
 theorem evalPrime_prime
-  (F : Formula)
+  (F : Formula_)
   (V : VarBoolAssignment)
   (h1 : F.IsPrime) :
   F.evalPrime V = V F :=
   by
   induction F
   case true_ | false_ | not_ | imp_ | and_ | or_ | iff_ =>
-    simp only [Formula.IsPrime] at h1
+    simp only [Formula_.IsPrime] at h1
   case pred_const_ | pred_var_ | eq_ | forall_ | exists_ | def_ =>
     rfl
 
 
 example
-  (F : Formula)
+  (F : Formula_)
   (V V' : VarBoolAssignment)
-  (h1 : ∀ H : Formula, H ∈ F.primeSet → V H = V' H) :
+  (h1 : ∀ H : Formula_, H ∈ F.primeSet → V H = V' H) :
   F.evalPrime V ↔ F.evalPrime V' :=
   by
   induction F
   case pred_const_ | pred_var_ | eq_ | forall_ | exists_ | def_ =>
-    simp only [Formula.primeSet] at h1
+    simp only [Formula_.primeSet] at h1
 
-    simp only [Formula.evalPrime]
+    simp only [Formula_.evalPrime]
     congr! 1
     apply h1
     simp
   case true_ | false_ =>
-    simp only [Formula.evalPrime]
+    simp only [Formula_.evalPrime]
   case not_ phi phi_ih =>
-    simp only [Formula.primeSet] at h1
+    simp only [Formula_.primeSet] at h1
 
-    simp only [Formula.evalPrime]
+    simp only [Formula_.evalPrime]
     congr! 1
     exact phi_ih h1
   case
@@ -173,10 +173,10 @@ example
   | and_ phi psi phi_ih psi_ih
   | or_ phi psi phi_ih psi_ih
   | iff_ phi psi phi_ih psi_ih =>
-    simp only [Formula.primeSet] at h1
+    simp only [Formula_.primeSet] at h1
     simp at h1
 
-    simp only [Formula.evalPrime]
+    simp only [Formula_.evalPrime]
     congr! 1
     · apply phi_ih
       intro H a1
@@ -191,51 +191,51 @@ example
 
 
 theorem evalPrime_substPrime_eq_evalPrime_evalPrime
-  (F : Formula)
-  (σ : Formula → Formula)
+  (F : Formula_)
+  (σ : Formula_ → Formula_)
   (V : VarBoolAssignment) :
   (F.substPrime σ).evalPrime V ↔
-    F.evalPrime fun H : Formula => (σ H).evalPrime V :=
+    F.evalPrime fun H : Formula_ => (σ H).evalPrime V :=
   by
   induction F
   case pred_const_ | pred_var_ | eq_ | forall_ | exists_ | def_ =>
-    simp only [Formula.substPrime]
-    simp only [Formula.evalPrime]
+    simp only [Formula_.substPrime]
+    simp only [Formula_.evalPrime]
     simp
   case true_ | false_ =>
     rfl
   case not_ phi phi_ih =>
-    simp only [Formula.substPrime]
-    simp only [Formula.evalPrime]
+    simp only [Formula_.substPrime]
+    simp only [Formula_.evalPrime]
     congr! 1
   case
       imp_ phi psi phi_ih psi_ih
     | and_ phi psi phi_ih psi_ih
     | or_ phi psi phi_ih psi_ih
     | iff_ phi psi phi_ih psi_ih =>
-    simp only [Formula.substPrime]
-    simp only [Formula.evalPrime]
+    simp only [Formula_.substPrime]
+    simp only [Formula_.evalPrime]
     congr! 1
 
 
 theorem isTautoPrime_imp_isTautoPrime_substPrime
-  (P : Formula)
+  (P : Formula_)
   (h1 : P.IsTautoPrime)
-  (σ : Formula → Formula) :
-  (Formula.substPrime σ P).IsTautoPrime :=
+  (σ : Formula_ → Formula_) :
+  (Formula_.substPrime σ P).IsTautoPrime :=
   by
-  simp only [Formula.IsTautoPrime] at h1
+  simp only [Formula_.IsTautoPrime] at h1
 
-  simp only [Formula.IsTautoPrime]
+  simp only [Formula_.IsTautoPrime]
   intro V
   simp only [evalPrime_substPrime_eq_evalPrime_evalPrime P σ V]
   apply h1
 
 
 example
-  (P Q R S : Formula)
+  (P Q R S : Formula_)
   (V : VarBoolAssignment)
-  (σ : Formula → Formula)
+  (σ : Formula_ → Formula_)
   (h1 : P.evalPrime V ↔ Q.evalPrime V) :
   (S.substPrime (Function.updateITE σ R P)).evalPrime V ↔
     (S.substPrime (Function.updateITE σ R Q)).evalPrime V :=
@@ -251,7 +251,7 @@ example
 
 
 theorem T_13_5
-  (P : Formula) :
+  (P : Formula_) :
   IsProof (P.imp_ P) :=
   by
   simp only [IsProof]
@@ -268,7 +268,7 @@ alias prop_id := T_13_5
 
 
 theorem T_13_6_no_deduct
-  (P Q : Formula) :
+  (P Q : Formula_) :
   IsProof (P.not_.imp_ (P.imp_ Q)) :=
   by
   apply IsDeduct.mp_ (P.not_.imp_ (Q.not_.imp_ P.not_))
@@ -285,10 +285,10 @@ theorem T_13_6_no_deduct
 
 
 theorem T_14_10
-  (F : Formula)
-  (Δ : Set Formula)
+  (F : Formula_)
+  (Δ : Set Formula_)
   (h1 : IsDeduct Δ F) :
-  ∀ Γ : Set Formula, IsDeduct (Δ ∪ Γ) F :=
+  ∀ Γ : Set Formula_, IsDeduct (Δ ∪ Γ) F :=
   by
   intro Γ
   induction h1
@@ -307,19 +307,19 @@ theorem T_14_10
 
 
 theorem T_14_10_comm
-  (Q : Formula)
-  (Δ : Set Formula)
+  (Q : Formula_)
+  (Δ : Set Formula_)
   (h1 : IsDeduct Δ Q) :
-  ∀ Γ : Set Formula, IsDeduct (Γ ∪ Δ) Q :=
+  ∀ Γ : Set Formula_, IsDeduct (Γ ∪ Δ) Q :=
   by
   simp only [Set.union_comm]
   exact T_14_10 Q Δ h1
 
 
 theorem C_14_11
-  (P : Formula)
+  (P : Formula_)
   (h1 : IsProof P) :
-  ∀ Δ : Set Formula, IsDeduct Δ P :=
+  ∀ Δ : Set Formula_, IsDeduct Δ P :=
   by
   intro Δ
   obtain s1 := T_14_10 P ∅ h1 Δ
@@ -331,8 +331,8 @@ alias proof_imp_deduct := C_14_11
 
 -- Deduction Theorem
 theorem T_14_3
-  (P Q : Formula)
-  (Δ : Set Formula)
+  (P Q : Formula_)
+  (Δ : Set Formula_)
   (h1 : IsDeduct (Δ ∪ {P}) Q) :
   IsDeduct Δ (P.imp_ Q) :=
   by
@@ -369,7 +369,7 @@ alias deduction_theorem := T_14_3
 
 
 theorem T_13_6
-  (P Q : Formula) :
+  (P Q : Formula_) :
   IsProof (P.not_.imp_ (P.imp_ Q)) :=
   by
   simp only [IsProof]
@@ -385,7 +385,7 @@ theorem T_13_6
 
 
 theorem T_14_5
-  (P : Formula) :
+  (P : Formula_) :
   IsProof (P.not_.not_.imp_ P) :=
   by
   simp only [IsProof]
@@ -404,7 +404,7 @@ theorem T_14_5
 
 
 theorem T_14_6
-  (P : Formula) :
+  (P : Formula_) :
   IsProof (P.imp_ P.not_.not_) :=
   by
   simp only [IsProof]
@@ -416,7 +416,7 @@ theorem T_14_6
 
 
 theorem T_14_7
-  (P Q : Formula) :
+  (P Q : Formula_) :
   IsProof ((P.imp_ Q).imp_ (Q.not_.imp_ P.not_)) :=
   by
   simp only [IsProof]
@@ -439,7 +439,7 @@ theorem T_14_7
 
 
 theorem T_14_8
-  (Q R : Formula) :
+  (Q R : Formula_) :
   IsProof (Q.imp_ (R.not_.imp_ (Q.imp_ R).not_)) :=
   by
   simp only [IsProof]
@@ -456,7 +456,7 @@ theorem T_14_8
 
 
 theorem T_14_9
-  (P S : Formula) :
+  (P S : Formula_) :
   IsProof ((S.imp_ P).imp_ ((S.not_.imp_ P).imp_ P)) :=
   by
   simp only [IsProof]
@@ -482,8 +482,8 @@ theorem T_14_9
 
 
 theorem deductionTheoremConverse
-  (P Q : Formula)
-  (Δ : Set Formula)
+  (P Q : Formula_)
+  (Δ : Set Formula_)
   (h1 : IsDeduct Δ (P.imp_ Q)) :
   IsDeduct (Δ ∪ {P}) Q :=
   by
@@ -494,8 +494,8 @@ theorem deductionTheoremConverse
 
 
 theorem T_14_12
-  (P Q : Formula)
-  (Δ Γ : Set Formula)
+  (P Q : Formula_)
+  (Δ Γ : Set Formula_)
   (h1 : IsDeduct Δ P)
   (h2 : IsDeduct Γ (P.imp_ Q)) :
   IsDeduct (Δ ∪ Γ) Q := by
@@ -507,8 +507,8 @@ theorem T_14_12
 
 
 theorem C_14_14
-  (P Q : Formula)
-  (Γ : Set Formula)
+  (P Q : Formula_)
+  (Γ : Set Formula_)
   (h1 : IsProof P)
   (h2 : IsDeduct Γ (P.imp_ Q)) :
   IsDeduct Γ Q := by
@@ -521,8 +521,8 @@ alias mp_proof_deduct := C_14_14
 
 
 theorem C_14_15
-  (P Q : Formula)
-  (Δ : Set Formula)
+  (P Q : Formula_)
+  (Δ : Set Formula_)
   (h1 : IsDeduct Δ P)
   (h2 : IsProof (P.imp_ Q)) :
   IsDeduct Δ Q := by
@@ -535,10 +535,10 @@ alias mp_deduct_proof := C_14_15
 
 
 theorem T_14_16
-  (F : Formula)
-  (Δ Γ : Set Formula)
+  (F : Formula_)
+  (Δ Γ : Set Formula_)
   (h1 : IsDeduct Γ F)
-  (h2 : ∀ H : Formula, H ∈ Γ → IsDeduct Δ H) :
+  (h2 : ∀ H : Formula_, H ∈ Γ → IsDeduct Δ H) :
   IsDeduct Δ F :=
   by
   induction h1
@@ -551,10 +551,10 @@ theorem T_14_16
 
 
 theorem C_14_17
-  (Q : Formula)
-  (Γ : Set Formula)
+  (Q : Formula_)
+  (Γ : Set Formula_)
   (h1 : IsDeduct Γ Q)
-  (h2 : ∀ P : Formula, P ∈ Γ → IsProof P) :
+  (h2 : ∀ P : Formula_, P ∈ Γ → IsProof P) :
   IsProof Q :=
   by
   simp only [IsProof] at h2
@@ -564,101 +564,101 @@ theorem C_14_17
 
 
 theorem eval_not
-  (P : Formula)
+  (P : Formula_)
   (V : VarBoolAssignment) :
-  Formula.evalPrime V (not_ P) ↔
-    ¬ Formula.evalPrime V P :=
+  Formula_.evalPrime V (not_ P) ↔
+    ¬ Formula_.evalPrime V P :=
   by
-  simp only [Formula.evalPrime]
+  simp only [Formula_.evalPrime]
 
 
 theorem eval_imp
-  (P Q : Formula)
+  (P Q : Formula_)
   (V : VarBoolAssignment) :
-  Formula.evalPrime V (imp_ P Q) ↔
-    (Formula.evalPrime V P → Formula.evalPrime V Q) :=
+  Formula_.evalPrime V (imp_ P Q) ↔
+    (Formula_.evalPrime V P → Formula_.evalPrime V Q) :=
   by
-  simp only [Formula.evalPrime]
+  simp only [Formula_.evalPrime]
 
 
 theorem eval_false
   (V : VarBoolAssignment) :
-  Formula.evalPrime V false_ ↔
+  Formula_.evalPrime V false_ ↔
     False :=
   by
-  simp only [Formula.evalPrime]
+  simp only [Formula_.evalPrime]
 
 
 theorem eval_and
-  (P Q : Formula)
+  (P Q : Formula_)
   (V : VarBoolAssignment) :
-  Formula.evalPrime V (and_ P Q) ↔
-    (Formula.evalPrime V P ∧ Formula.evalPrime V Q) :=
+  Formula_.evalPrime V (and_ P Q) ↔
+    (Formula_.evalPrime V P ∧ Formula_.evalPrime V Q) :=
   by
-  simp only [Formula.evalPrime]
+  simp only [Formula_.evalPrime]
 
 
 theorem eval_or
-  (P Q : Formula)
+  (P Q : Formula_)
   (V : VarBoolAssignment) :
-  Formula.evalPrime V (or_ P Q) ↔
-    (Formula.evalPrime V P ∨ Formula.evalPrime V Q) :=
+  Formula_.evalPrime V (or_ P Q) ↔
+    (Formula_.evalPrime V P ∨ Formula_.evalPrime V Q) :=
   by
-  simp only [Formula.evalPrime]
+  simp only [Formula_.evalPrime]
 
 
 theorem eval_iff
-  (P Q : Formula)
+  (P Q : Formula_)
   (V : VarBoolAssignment) :
-  Formula.evalPrime V (iff_ P Q) ↔
-    (Formula.evalPrime V P ↔ Formula.evalPrime V Q) :=
+  Formula_.evalPrime V (iff_ P Q) ↔
+    (Formula_.evalPrime V P ↔ Formula_.evalPrime V Q) :=
   by
-  simp only [Formula.evalPrime]
+  simp only [Formula_.evalPrime]
 
 
 theorem is_tauto_prop_true :
   true_.IsTautoPrime :=
   by
-  simp only [Formula.IsTautoPrime]
-  simp only [Formula.evalPrime]
+  simp only [Formula_.IsTautoPrime]
+  simp only [Formula_.evalPrime]
   simp
 
 
 theorem is_tauto_prop_1
-  (P Q : Formula) :
+  (P Q : Formula_) :
   (P.imp_ (Q.imp_ P)).IsTautoPrime :=
   by
-  simp only [Formula.IsTautoPrime]
+  simp only [Formula_.IsTautoPrime]
   tauto
 
 
 theorem is_tauto_prop_2
-  (P Q R : Formula) :
+  (P Q R : Formula_) :
   ((P.imp_ (Q.imp_ R)).imp_ ((P.imp_ Q).imp_ (P.imp_ R))).IsTautoPrime :=
   by
-  simp only [Formula.IsTautoPrime]
+  simp only [Formula_.IsTautoPrime]
   tauto
 
 
 theorem is_tauto_prop_3
-  (P Q : Formula) :
+  (P Q : Formula_) :
   (((not_ P).imp_ (not_ Q)).imp_ (Q.imp_ P)).IsTautoPrime :=
   by
-  simp only [Formula.IsTautoPrime]
+  simp only [Formula_.IsTautoPrime]
   simp only [eval_not, eval_imp]
   tauto
 
 
 theorem is_tauto_mp
-  (P Q : Formula)
+  (P Q : Formula_)
   (h1 : (P.imp_ Q).IsTautoPrime)
   (h2 : P.IsTautoPrime) :
   Q.IsTautoPrime :=
   by
-  simp only [Formula.IsTautoPrime] at h1
+  simp only [Formula_.IsTautoPrime] at h1
   simp only [eval_imp] at h1
 
-  simp only [Formula.IsTautoPrime] at h2
+  simp only [Formula_.IsTautoPrime] at h2
 
   tauto
 
@@ -666,31 +666,31 @@ theorem is_tauto_mp
 theorem is_tauto_def_false :
   (false_.iff_ (not_ true_)).IsTautoPrime :=
   by
-  simp only [Formula.IsTautoPrime]
+  simp only [Formula_.IsTautoPrime]
   simp only [eval_not, eval_iff]
   tauto
 
 theorem is_tauto_def_and
-  (P Q : Formula) :
+  (P Q : Formula_) :
   ((P.and_ Q).iff_ (not_ (P.imp_ (not_ Q)))).IsTautoPrime :=
   by
-  simp only [Formula.IsTautoPrime]
+  simp only [Formula_.IsTautoPrime]
   simp only [eval_and, eval_not, eval_imp, eval_iff]
   tauto
 
 theorem is_tauto_def_or
-  (P Q : Formula) :
+  (P Q : Formula_) :
   ((P.or_ Q).iff_ ((not_ P).imp_ Q)).IsTautoPrime :=
   by
-  simp only [Formula.IsTautoPrime]
+  simp only [Formula_.IsTautoPrime]
   simp only [eval_or, eval_not, eval_imp, eval_iff]
   tauto
 
 theorem is_tauto_def_iff
-  (P Q : Formula) :
+  (P Q : Formula_) :
   (not_ (((P.iff_ Q).imp_ (not_ ((P.imp_ Q).imp_ (not_ (Q.imp_ P))))).imp_ (not_ ((not_ ((P.imp_ Q).imp_ (not_ (Q.imp_ P)))).imp_ (P.iff_ Q))))).IsTautoPrime :=
   by
-  simp only [Formula.IsTautoPrime]
+  simp only [Formula_.IsTautoPrime]
   simp only [eval_iff, eval_not, eval_imp]
   tauto
 
@@ -699,7 +699,7 @@ theorem is_tauto_def_iff
   Proof of the soundness of classical propositional logic.
 -/
 example
-  (F : Formula)
+  (F : Formula_)
   (h1 : IsPropProof F) :
   F.IsTautoPrime :=
   by
@@ -729,52 +729,52 @@ example
 
 
 theorem mem_primeSet_isPrime
-  (F F' : Formula)
+  (F F' : Formula_)
   (h1 : F' ∈ F.primeSet) :
   F'.IsPrime :=
   by
   induction F
   case pred_const_ | pred_var_ =>
-    simp only [Formula.primeSet] at h1
+    simp only [Formula_.primeSet] at h1
     simp at h1
     subst h1
-    simp only [Formula.IsPrime]
+    simp only [Formula_.IsPrime]
   case true_ | false_ =>
-    simp only [Formula.primeSet] at h1
+    simp only [Formula_.primeSet] at h1
     simp at h1
   case eq_ x y =>
-    simp only [Formula.primeSet] at h1
+    simp only [Formula_.primeSet] at h1
     simp at h1
     subst h1
-    simp only [Formula.IsPrime]
+    simp only [Formula_.IsPrime]
   case not_ phi phi_ih =>
-    simp only [Formula.primeSet] at h1
+    simp only [Formula_.primeSet] at h1
     exact phi_ih h1
   case
       imp_ phi psi phi_ih psi_ih
     | and_ phi psi phi_ih psi_ih
     | or_ phi psi phi_ih psi_ih
     | iff_ phi psi phi_ih psi_ih =>
-    simp only [Formula.primeSet] at h1
+    simp only [Formula_.primeSet] at h1
     simp at h1
     tauto
   case forall_ x phi | exists_ x phi =>
-    simp only [Formula.primeSet] at h1
+    simp only [Formula_.primeSet] at h1
     simp at h1
     subst h1
-    simp only [Formula.IsPrime]
+    simp only [Formula_.IsPrime]
   case def_ =>
-    simp only [Formula.primeSet] at h1
+    simp only [Formula_.primeSet] at h1
     simp at h1
     subst h1
-    simp only [Formula.IsPrime]
+    simp only [Formula_.IsPrime]
 
 
 theorem L_15_7
-  (F F' : Formula)
-  (Δ_U : Set Formula)
+  (F F' : Formula_)
+  (Δ_U : Set Formula_)
   (V : VarBoolAssignment)
-  (Δ_U' : Set Formula)
+  (Δ_U' : Set Formula_)
   (h1 : F.primeSet.toSet ⊆ Δ_U)
   (h2 : Δ_U' = Δ_U.image (evalPrimeFfToNot V))
   (h3 : F' = evalPrimeFfToNot V F) :
@@ -785,33 +785,33 @@ theorem L_15_7
   induction F
   case pred_const_ X xs =>
     let F := pred_const_ X xs
-    simp only [Formula.primeSet] at h1
+    simp only [Formula_.primeSet] at h1
     simp at h1
 
     simp only [evalPrimeFfToNot]
-    simp only [Formula.evalPrime]
+    simp only [Formula_.evalPrime]
     apply IsDeduct.assume_
     simp
     apply Exists.intro F
     tauto
   case pred_var_ X xs =>
     let F := pred_var_ X xs
-    simp only [Formula.primeSet] at h1
+    simp only [Formula_.primeSet] at h1
     simp at h1
 
     simp only [evalPrimeFfToNot]
-    simp only [Formula.evalPrime]
+    simp only [Formula_.evalPrime]
     apply IsDeduct.assume_
     simp
     apply Exists.intro F
     tauto
   case eq_ x y =>
     let F := eq_ x y
-    simp only [Formula.primeSet] at h1
+    simp only [Formula_.primeSet] at h1
     simp at h1
 
     simp only [evalPrimeFfToNot]
-    simp only [Formula.evalPrime]
+    simp only [Formula_.evalPrime]
     apply IsDeduct.assume_
     simp
     apply Exists.intro F
@@ -820,15 +820,15 @@ theorem L_15_7
     apply IsDeduct.axiom_
     apply IsAxiom.prop_true_
   case false_ =>
-    simp only [Formula.primeSet] at h1
+    simp only [Formula_.primeSet] at h1
     simp at h1
 
     simp only [evalPrimeFfToNot]
-    simp only [Formula.evalPrime]
+    simp only [Formula_.evalPrime]
     simp
     sorry
   case not_ phi phi_ih =>
-    simp only [Formula.primeSet] at h1
+    simp only [Formula_.primeSet] at h1
 
     simp only [evalPrimeFfToNot] at phi_ih
 
@@ -848,7 +848,7 @@ theorem L_15_7
       simp at phi_ih
       exact phi_ih h1
   case imp_ phi psi phi_ih psi_ih =>
-    simp only [Formula.primeSet] at h1
+    simp only [Formula_.primeSet] at h1
     simp at h1
 
     simp only [evalPrimeFfToNot] at phi_ih
@@ -892,22 +892,22 @@ theorem L_15_7
   case forall_ x phi phi_ih =>
     let F := forall_ x phi
 
-    simp only [Formula.primeSet] at h1
+    simp only [Formula_.primeSet] at h1
     simp at h1
 
     simp only [evalPrimeFfToNot]
-    simp only [Formula.evalPrime]
+    simp only [Formula_.evalPrime]
     apply IsDeduct.assume_
     simp
     apply Exists.intro F
     tauto
   case def_ X xs =>
     let F := def_ X xs
-    simp only [Formula.primeSet] at h1
+    simp only [Formula_.primeSet] at h1
     simp at h1
 
     simp only [evalPrimeFfToNot]
-    simp only [Formula.evalPrime]
+    simp only [Formula_.evalPrime]
     apply IsDeduct.assume_
     simp
     apply Exists.intro F
@@ -917,8 +917,8 @@ theorem L_15_7
 
 
 theorem T_14_9_Deduct
-  (P U : Formula)
-  (Δ : Set Formula)
+  (P U : Formula_)
+  (Δ : Set Formula_)
   (h1 : IsDeduct (Δ ∪ {U}) P)
   (h2 : IsDeduct (Δ ∪ {U.not_}) P) :
   IsDeduct Δ P :=
@@ -934,7 +934,7 @@ theorem T_14_9_Deduct
 
 
 theorem evalPrimeFfToNot_of_function_updateIte_true
-  (F F' : Formula)
+  (F F' : Formula_)
   (V : VarBoolAssignment)
   (h1 : F.IsPrime) :
   evalPrimeFfToNot (Function.updateITE V F' true) F =
@@ -944,14 +944,14 @@ theorem evalPrimeFfToNot_of_function_updateIte_true
   case pred_const_ | pred_var_ | eq_ | forall_ | exists_ | def_ =>
     unfold Function.updateITE
     simp only [evalPrimeFfToNot]
-    simp only [Formula.evalPrime]
+    simp only [Formula_.evalPrime]
     split_ifs <;> tauto
   case true_ | false_ | not_ | imp_ | and_ | or_ | iff_ =>
-    simp only [Formula.IsPrime] at h1
+    simp only [Formula_.IsPrime] at h1
 
 
 theorem evalPrimeFfToNot_of_function_updateIte_false
-  (F F' : Formula)
+  (F F' : Formula_)
   (V : VarBoolAssignment)
   (h1 : F.IsPrime) :
   evalPrimeFfToNot (Function.updateITE V F' false) F =
@@ -961,18 +961,18 @@ theorem evalPrimeFfToNot_of_function_updateIte_false
   case pred_const_ | pred_var_ | eq_ | forall_ | exists_ | def_ =>
     unfold Function.updateITE
     simp only [evalPrimeFfToNot]
-    simp only [Formula.evalPrime]
+    simp only [Formula_.evalPrime]
     split_ifs <;> tauto
   case true_ | false_ | not_ | imp_ | and_ | or_ | iff_ =>
-    simp only [Formula.IsPrime] at h1
+    simp only [Formula_.IsPrime] at h1
 
 
 theorem image_of_evalPrimeFfToNot_of_function_updateIte
-  (U : Formula)
-  (Δ : Set Formula)
+  (U : Formula_)
+  (Δ : Set Formula_)
   (V : VarBoolAssignment)
   (b : Bool)
-  (h1_Δ : ∀ U' : Formula, U' ∈ Δ → U'.IsPrime)
+  (h1_Δ : ∀ U' : Formula_, U' ∈ Δ → U'.IsPrime)
   (h1_U : U.IsPrime)
   (h2 : U ∉ Δ) :
   Δ.image (evalPrimeFfToNot (Function.updateITE V U b)) =
@@ -997,9 +997,9 @@ theorem image_of_evalPrimeFfToNot_of_function_updateIte
 
 
 theorem propCompleteAuxAux
-  (P U : Formula)
-  (Δ : Set Formula)
-  (h1_Δ : ∀ U' : Formula, U' ∈ Δ → U'.IsPrime)
+  (P U : Formula_)
+  (Δ : Set Formula_)
+  (h1_Δ : ∀ U' : Formula_, U' ∈ Δ → U'.IsPrime)
   (h1_U : U.IsPrime)
   (h2 : U ∉ Δ)
   (h3 : ∀ V : VarBoolAssignment, IsDeduct (Δ.image (evalPrimeFfToNot V) ∪ {evalPrimeFfToNot V U}) P) :
@@ -1022,8 +1022,8 @@ theorem propCompleteAuxAux
 
 
 theorem propCompleteAux
-  (P : Formula)
-  (Δ_U : Finset Formula)
+  (P : Formula_)
+  (Δ_U : Finset Formula_)
   (h1 : Δ_U ⊆ P.primeSet)
   (h2 : ∀ V : VarBoolAssignment, IsDeduct (Δ_U.image (evalPrimeFfToNot V)) P) :
   IsDeduct ∅ P :=
@@ -1061,7 +1061,7 @@ theorem propCompleteAux
   Proof of the completeness of classical propositional logic.
 -/
 theorem prop_complete
-  (P : Formula)
+  (P : Formula_)
   (h1 : P.IsTautoPrime) :
   IsProof P :=
   by
@@ -1072,7 +1072,7 @@ theorem prop_complete
     apply L_15_7 P P P.primeSet V (P.primeSet.image (evalPrimeFfToNot V))
     · rfl
     · simp only [Finset.coe_image]
-    · simp only [Formula.IsTautoPrime] at h1
+    · simp only [Formula_.IsTautoPrime] at h1
       simp only [evalPrimeFfToNot]
       specialize h1 V
       simp only [if_pos h1]
@@ -1081,7 +1081,7 @@ theorem prop_complete
 macro "SC" : tactic => `(tactic|(
   apply proof_imp_deduct
   apply prop_complete
-  simp only [Formula.IsTautoPrime]
+  simp only [Formula_.IsTautoPrime]
   simp only [eval_not, eval_imp]
   tauto))
 
